made rather a mess trying to get andy's metric stuff to work; commiting so I can ask andres for help

bedrock2/src/bedrock2/WeakestPrecondition.v
@@ -1,6 +1,7 @@
 Require Import coqutil.Macros.subst coqutil.Macros.unique bedrock2.Notations coqutil.Map.Interface coqutil.Map.OfListWord.
 Require Import Coq.ZArith.BinIntDef coqutil.Word.Interface coqutil.Word.Bitwidth.
 Require Import coqutil.dlet bedrock2.Syntax bedrock2.Semantics.
+Require Import bedrock2.MetricLogging.
 
 Section WeakestPrecondition.
   Context {width: Z} {BW: Bitwidth width} {word: word.word width} {mem: map.map word Byte.byte}.
@@ -9,140 +10,156 @@ Section WeakestPrecondition.
   Context {ext_spec: ExtSpec}.
   Implicit Types (t : trace) (m : mem) (l : locals).
 
-  Definition literal v (post : word -> Prop) : Prop :=
-    dlet! v := word.of_Z v in post v.
-  Definition get (l : locals) (x : String.string) (post : word -> Prop) : Prop :=
-    bind_ex_Some v <- map.get l x; post v.
-  Definition load s m a (post : _ -> Prop) : Prop :=
-    bind_ex_Some v <- load s m a; post v.
+Local Notation metrics := MetricLog.
+
+  Definition literal v mc (post : (word * metrics) -> Prop) : Prop :=
+    dlet! v := word.of_Z v in post (v, addMetricInstructions 8 (addMetricLoads 8 mc)).
+  Definition get (l : locals) (x : String.string) mc (post : (word * metrics) -> Prop) : Prop :=
+    bind_ex_Some v <- map.get l x; post (v, addMetricInstructions 1 (addMetricLoads 2 mc)).
+  Definition load s m a mc (post : (word * metrics) -> Prop) : Prop :=
+    bind_ex_Some v <- load s m a; post (v, addMetricInstructions 1 (addMetricLoads 2 mc)).
   Definition store sz m a v post :=
     bind_ex_Some m <- store sz m a v; post m.
 
   Section WithMemAndLocals.
     Context (m : mem) (l : locals).
-    Definition expr_body rec (e : Syntax.expr) (post : word -> Prop) : Prop :=
+    Definition expr_body (rec : _->_->(word*metrics->Prop)->Prop) (e : Syntax.expr) (mc : metrics) (post : word * metrics -> Prop) : Prop :=
       match e with
       | expr.literal v =>
-        literal v post
+        literal v mc post
       | expr.var x =>
-        get l x post
+        get l x mc post
       | expr.op op e1 e2 =>
-        rec e1 (fun v1 =>
-        rec e2 (fun v2 =>
-        post (interp_binop op v1 v2)))
+        rec e1 mc (fun '(v1, mc') =>
+        rec e2 mc' (fun '(v2, mc'') =>
+        post (interp_binop op v1 v2, addMetricInstructions 2 (addMetricLoads 2 mc''))))
       | expr.load s e =>
-        rec e (fun a =>
-        load s m a post)
+       rec e mc (fun '(a, mc') =>
+        load s m a mc' post)
       | expr.inlinetable s t e =>
-        rec e (fun a =>
-        load s (map.of_list_word t) a post)
+         rec e mc (fun '(a, mc') =>
+        load s (map.of_list_word t) a (addMetricInstructions 2
+                                      (addMetricLoads 2
+                                      (addMetricJumps 1 mc'))) post)
       | expr.ite c e1 e2 =>
-        rec c (fun b => rec (if word.eqb b (word.of_Z 0) then e2 else e1) post)
+        rec c mc (fun '(b, mc') => rec (if word.eqb b (word.of_Z 0) then e2 else e1) (addMetricInstructions 2 (addMetricLoads 2 (addMetricJumps 1 mc'))) post) 
     end.
     Fixpoint expr e := expr_body expr e.
   End WithMemAndLocals.
 
   Section WithF.
-    Context {A B} (f: A -> (B -> Prop) -> Prop).
-    Definition list_map_body rec (xs : list A) (post : list B -> Prop) : Prop :=
+    Context {A B} (f: A -> metrics -> (B * metrics -> Prop) -> Prop).
+    Definition list_map_body rec (xs : list A) (mc : metrics) (post : list B * metrics -> Prop) : Prop :=
       match xs with
-      | nil => post nil
+      | nil => post (nil, mc)
       | cons x xs' =>
-        f x (fun y =>
-        rec xs' (fun ys' =>
-        post (cons y ys')))
+        f x mc (fun '(y, mc') =>
+        rec xs' mc' (fun '(ys', mc'') =>
+        post (cons y ys', mc'')))
       end.
     Fixpoint list_map xs := list_map_body list_map xs.
   End WithF.
 
   Section WithFunctions.
-    Context (call : String.string -> trace -> mem -> list word -> (trace -> mem -> list word -> Prop) -> Prop).
-    Definition dexpr m l e v := expr m l e (eq v).
-    Definition dexprs m l es vs := list_map (expr m l) es (eq vs).
-    Definition cmd_body (rec:_->_->_->_->_->Prop) (c : cmd) (t : trace) (m : mem) (l : locals)
-             (post : trace -> mem -> locals -> Prop) : Prop :=
+    Context (call : String.string -> trace -> mem -> list word -> metrics -> (trace -> mem -> list word -> metrics -> Prop) -> Prop).
+    Definition dexpr m l e mc vmc := expr m l e mc (eq vmc).
+    Definition dexprs m l es mc vmcs := list_map (expr m l) es mc (eq vmcs).
+    Definition cmd_body (rec:_->_->_->_->_->_->Prop) (c : cmd) (t : trace) (m : mem) (l : locals) (mc : metrics)
+             (post : trace -> mem -> locals -> metrics -> Prop) : Prop :=
       (* give value of each pure expression when stating its subproof *)
       match c with
-      | cmd.skip => post t m l
+      | cmd.skip => post t m l mc
       | cmd.set x ev =>
-        bind_ex v <- dexpr m l ev;
+        bind_ex_pair (v, mc') <- dexpr m l ev mc;
         dlet! l := map.put l x v in
-        post t m l
+        post t m l (addMetricInstructions 1 (addMetricLoads 1 mc'))
       | cmd.unset x =>
         dlet! l := map.remove l x in
-        post t m l
+        post t m l mc
       | cmd.store sz ea ev =>
-        bind_ex a <- dexpr m l ea;
-        bind_ex v <- dexpr m l ev;
+        bind_ex_pair (a, mc') <- dexpr m l ea mc;
+        bind_ex_pair (v, mc'') <- dexpr m l ev mc';
         store sz m a v (fun m =>
-        post t m l)
+        post t m l (addMetricInstructions 1 (addMetricLoads 1 (addMetricStores 1 mc''))))
       | cmd.stackalloc x n c =>
         Z.modulo n (bytes_per_word width) = 0 /\
         forall a mStack mCombined,
           anybytes a n mStack -> map.split mCombined m mStack ->
           dlet! l := map.put l x a in
-          rec c t mCombined l (fun t' mCombined' l' =>
+          rec c t mCombined l (addMetricInstructions 1 (addMetricLoads 1 mc))
+          (fun t' mCombined' l' mc' =>
           exists m' mStack',
           anybytes a n mStack' /\ map.split mCombined' m' mStack' /\
-          post t' m' l')
+          post t' m' l' mc')
       | cmd.cond br ct cf =>
-        bind_ex v <- dexpr m l br;
-        (word.unsigned v <> 0%Z -> rec ct t m l post) /\
-        (word.unsigned v = 0%Z -> rec cf t m l post)
+        bind_ex_pair (v, mc') <- dexpr m l br mc;
+        dlet! mc'' := addMetricInstructions 2 (addMetricLoads 2 (addMetricJumps 1 mc')) in
+        (word.unsigned v <> 0%Z -> rec ct t m l mc'' post) /\
+        (word.unsigned v = 0%Z -> rec cf t m l mc'' post)
       | cmd.seq c1 c2 =>
-        rec c1 t m l (fun t m l => rec c2 t m l post)
+        rec c1 t m l mc (fun t m l mc => rec c2 t m l mc post)
       | cmd.while e c =>
-        exists measure (lt:measure->measure->Prop) (inv:measure->trace->mem->locals->Prop),
+        exists measure (lt:measure->measure->Prop) (inv:measure->trace->mem->locals->metrics->Prop),
         Coq.Init.Wf.well_founded lt /\
-        (exists v, inv v t m l) /\
-        (forall v t m l, inv v t m l ->
-          bind_ex b <- dexpr m l e;
-          (word.unsigned b <> 0%Z -> rec c t m l (fun t' m l =>
-            exists v', inv v' t' m l /\ lt v' v)) /\
-          (word.unsigned b = 0%Z -> post t m l))
+        (exists v, inv v t m l mc) /\
+        (forall v t m l mc, inv v t m l mc ->
+          bind_ex_pair (b, mc') <- dexpr m l e mc;
+          (word.unsigned b <> 0%Z -> rec c t m l mc' (fun t' m' l' mc'' =>
+            exists v', inv v' t' m' l' (addMetricInstructions 2
+                                       (addMetricLoads 2
+                                       (addMetricJumps 1 mc''))) /\ lt v' v)) /\
+          (word.unsigned b = 0%Z -> post t m l (addMetricInstructions 1
+                                               (addMetricLoads 1
+                                               (addMetricJumps 1 mc')))))
       | cmd.call binds fname arges =>
-        bind_ex args <- dexprs m l arges;
-        call fname t m args (fun t m rets =>
+        bind_ex_pair (args, mc') <- dexprs m l arges mc;
+        call fname t m args mc' (fun t m rets mc'' =>
           bind_ex_Some l <- map.putmany_of_list_zip binds rets l;
-          post t m l)
+          post t m l (addMetricInstructions 100 (addMetricJumps 100 (addMetricLoads 100 (addMetricStores 100 mc'')))))
       | cmd.interact binds action arges =>
-        bind_ex args <- dexprs m l arges;
+        bind_ex_pair (args, mc') <- dexprs m l arges mc;
         exists mKeep mGive, map.split m mKeep mGive /\
         ext_spec t mGive action args (fun mReceive rets =>
           bind_ex_Some l' <- map.putmany_of_list_zip binds rets l;
           forall m', map.split m' mKeep mReceive ->
-          post (cons ((mGive, action, args), (mReceive, rets)) t) m' l')
+          post (cons ((mGive, action, args), (mReceive, rets)) t) m' l' (addMetricInstructions 1
+                                                                        (addMetricStores 1
+                                                                        (addMetricLoads 2 mc'))))
       end.
     Fixpoint cmd c := cmd_body cmd c.
   End WithFunctions.
 
-  Definition func call '(innames, outnames, c) (t : trace) (m : mem) (args : list word) (post : trace -> mem -> list word -> Prop) :=
+Definition func call '(innames, outnames, c) (t : trace) (m : mem) (args : list word) (mc : metrics) (post : trace -> mem -> list word -> metrics -> Prop) :=
       bind_ex_Some l <- map.of_list_zip innames args;
-      cmd call c t m l (fun t m l =>
-        list_map (get l) outnames (fun rets =>
-        post t m rets)).
+      cmd call c t m l mc (fun t m l mc =>
+        (* this list_map is only used proof-side and not actually executed in the program, so ignore the new metrics *)
+        list_map (get l) outnames mc (fun '(rets, _) =>
+                                        post t m rets mc
+
+        )).
+
 
   Definition call_body rec (functions : list (String.string * (list String.string * list String.string * cmd.cmd)))
-                (fname : String.string) (t : trace) (m : mem) (args : list word)
-                (post : trace -> mem -> list word -> Prop) : Prop :=
+                (fname : String.string) (t : trace) (m : mem) (args : list word) (mc: metrics)
+                (post : trace -> mem -> list word -> metrics -> Prop) : Prop :=
     match functions with
     | nil => False
     | cons (f, decl) functions =>
       if String.eqb f fname
-      then func (rec functions) decl t m args post
-      else rec functions fname t m args post
+      then func (rec functions) decl t m args mc post
+      else rec functions fname t m args mc post
     end.
   Fixpoint call functions := call_body call functions.
 
-  Definition program funcs main t m l post : Prop := cmd (call funcs) main t m l post.
+  Definition program funcs main t m l mc post : Prop := cmd (call funcs) main t m l mc post.
 End WeakestPrecondition.
 
 Ltac unfold1_cmd e :=
   lazymatch e with
-    @cmd ?width ?BW ?word ?mem ?locals ?ext_spec ?CA ?c ?t ?m ?l ?post =>
+    @cmd ?width ?BW ?word ?mem ?locals ?ext_spec ?CA ?c ?t ?m ?l ?mc ?post =>
     let c := eval hnf in c in
     constr:(@cmd_body width BW word mem locals ext_spec CA
-                      (@cmd width BW word mem locals ext_spec CA) c t m l post)
+                      (@cmd width BW word mem locals ext_spec CA) c t m l mc post)
   end.
 Ltac unfold1_cmd_goal :=
   let G := lazymatch goal with |- ?G => G end in
@@ -151,9 +168,9 @@ Ltac unfold1_cmd_goal :=
 
 Ltac unfold1_expr e :=
   lazymatch e with
-    @expr ?width ?word ?mem ?locals ?m ?l ?arg ?post =>
+    @expr ?width ?word ?mem ?locals ?m ?l ?arg ?mc ?post =>
     let arg := eval hnf in arg in
-    constr:(@expr_body width word mem locals m l (@expr width word mem locals m l) arg post)
+    constr:(@expr_body width word mem locals m l (@expr width word mem locals m l) arg mc post)
   end.
 Ltac unfold1_expr_goal :=
   let G := lazymatch goal with |- ?G => G end in
@@ -162,9 +179,9 @@ Ltac unfold1_expr_goal :=
 
 Ltac unfold1_list_map e :=
   lazymatch e with
-    @list_map ?A ?B ?P ?arg ?post =>
+    @list_map ?A ?B ?P ?arg ?mc ?post =>
     let arg := eval hnf in arg in
-    constr:(@list_map_body A B P (@list_map A B P) arg post)
+    constr:(@list_map_body A B P (@list_map A B P) arg mc post)
   end.
 Ltac unfold1_list_map_goal :=
   let G := lazymatch goal with |- ?G => G end in
@@ -173,10 +190,10 @@ Ltac unfold1_list_map_goal :=
 
 Ltac unfold1_call e :=
   lazymatch e with
-    @call ?width ?BW ?word ?mem ?locals ?ext_spec ?fs ?fname ?t ?m ?l ?post =>
+    @call ?width ?BW ?word ?mem ?locals ?ext_spec ?fs ?fname ?t ?m ?l ?mc ?post =>
     let fs := eval hnf in fs in
     constr:(@call_body width BW word mem locals ext_spec
-                       (@call width BW word mem locals ext_spec) fs fname t m l post)
+                       (@call width BW word mem locals ext_spec) fs fname t m l mc post)
   end.
 Ltac unfold1_call_goal :=
   let G := lazymatch goal with |- ?G => G end in
@@ -185,17 +202,17 @@ Ltac unfold1_call_goal :=
 
 Import Coq.ZArith.ZArith.
 
-Notation "'fnspec!' name a0 .. an '/' g0 .. gn '~>' r0 .. rn ',' '{' 'requires' tr mem := pre ';' 'ensures' tr' mem' ':=' post '}'" :=
+Notation "'fnspec!' name a0 .. an '/' g0 .. gn '~>' r0 .. rn ',' '{' 'requires' tr mem mc := pre ';' 'ensures' tr' mem' mc' ':=' post '}'" :=
   (fun functions =>
      (forall a0,
         .. (forall an,
               (forall g0,
                   .. (forall gn,
-                         (forall tr mem,
+                         (forall tr mem mc,
                              pre ->
                              WeakestPrecondition.call
-                               functions name tr mem (cons a0 .. (cons an nil) ..)
-                               (fun tr' mem' rets =>
+                               functions name tr mem (cons a0 .. (cons an nil) ..) mc
+                               (fun tr' mem' rets mc' =>
                                   (exists r0,
                                       .. (exists rn,
                                              rets = (cons r0 .. (cons rn nil) ..) /\
@@ -205,39 +222,39 @@ Notation "'fnspec!' name a0 .. an '/' g0 .. gn '~>' r0 .. rn ',' '{' 'requires' 
      a0 binder, an binder,
      g0 binder, gn binder,
      r0 closed binder, rn closed binder,
-     tr name, tr' name, mem name, mem' name,
+     tr name, tr' name, mem name, mem' name, mc name, mc' name,
      pre at level 200,
      post at level 200).
 
-Notation "'fnspec!' name a0 .. an '/' g0 .. gn ',' '{' 'requires' tr mem := pre ';' 'ensures' tr' mem' ':=' post '}'" :=
+Notation "'fnspec!' name a0 .. an '/' g0 .. gn ',' '{' 'requires' tr mem mc := pre ';' 'ensures' tr' mem' mc' ':=' post '}'" :=
   (fun functions =>
      (forall a0,
         .. (forall an,
               (forall g0,
                   .. (forall gn,
-                         (forall tr mem,
+                         (forall tr mem mc,
                              pre ->
                              WeakestPrecondition.call
-                               functions name tr mem (cons a0 .. (cons an nil) ..)
-                               (fun tr' mem' rets =>
+                               functions name tr mem (cons a0 .. (cons an nil) ..) mc
+                               (fun tr' mem' rets mc' =>
                                   rets = nil /\ post))) ..)) ..))
     (at level 200,
      name at level 0,
      a0 binder, an binder,
      g0 binder, gn binder,
-     tr name, tr' name, mem name, mem' name,
+     tr name, tr' name, mem name, mem' name, mc name, mc' name,
      pre at level 200,
      post at level 200).
 
-Notation "'fnspec!' name a0 .. an '~>' r0 .. rn ',' '{' 'requires' tr mem := pre ';' 'ensures' tr' mem' ':=' post '}'" :=
+Notation "'fnspec!' name a0 .. an '~>' r0 .. rn ',' '{' 'requires' tr mem mc := pre ';' 'ensures' tr' mem' mc' ':=' post '}'" :=
   (fun functions =>
      (forall a0,
         .. (forall an,
-               (forall tr mem,
+               (forall tr mem mc,
                    pre ->
                    WeakestPrecondition.call
-                     functions name tr mem (cons a0 .. (cons an nil) ..)
-                     (fun tr' mem' rets =>
+                     functions name tr mem (cons a0 .. (cons an nil) ..) mc
+                     (fun tr' mem' rets mc' =>
                         (exists r0,
                             .. (exists rn,
                                    rets = (cons r0 .. (cons rn nil) ..) /\
@@ -246,20 +263,20 @@ Notation "'fnspec!' name a0 .. an '~>' r0 .. rn ',' '{' 'requires' tr mem := pre
      name at level 0,
      a0 binder, an binder,
      r0 closed binder, rn closed binder,
-     tr name, tr' name, mem name, mem' name,
+     tr name, tr' name, mem name, mem' name, mc name, mc' name,
      pre at level 200,
      post at level 200).
 
-Notation "'fnspec!' name '/' g0 .. gn '~>' r0 .. rn ',' '{' 'requires' tr mem := pre ';' 'ensures' tr' mem' ':=' post '}'" :=
+Notation "'fnspec!' name '/' g0 .. gn '~>' r0 .. rn ',' '{' 'requires' tr mem mc := pre ';' 'ensures' tr' mem' mc' ':=' post '}'" :=
   (fun functions =>
         (forall an,
               (forall g0,
                   .. (forall gn,
-                         (forall tr mem,
+                         (forall tr mem mc,
                              pre ->
                              WeakestPrecondition.call
-                               functions name tr mem nil
-                               (fun tr' mem' rets =>
+                               functions name tr mem nil mc
+                               (fun tr' mem' rets mc' =>
                                   (exists r0,
                                       .. (exists rn,
                                              rets = (cons r0 .. (cons rn nil) ..) /\
@@ -268,51 +285,51 @@ Notation "'fnspec!' name '/' g0 .. gn '~>' r0 .. rn ',' '{' 'requires' tr mem :=
      name at level 0,
      g0 binder, gn binder,
      r0 closed binder, rn closed binder,
-     tr name, tr' name, mem name, mem' name,
+     tr name, tr' name, mem name, mem' name, mc name, mc' name,
      pre at level 200,
      post at level 200).
 
-Notation "'fnspec!' name a0 .. an ',' '{' 'requires' tr mem := pre ';' 'ensures' tr' mem' ':=' post '}'" :=
+Notation "'fnspec!' name a0 .. an ',' '{' 'requires' tr mem mc := pre ';' 'ensures' tr' mem' mc' ':=' post '}'" :=
   (fun functions =>
      (forall a0,
         .. (forall an,
-               (forall tr mem,
+               (forall tr mem mc,
                    pre ->
                    WeakestPrecondition.call
-                     functions name tr mem (cons a0 .. (cons an nil) ..)
-                     (fun tr' mem' rets =>
+                     functions name tr mem (cons a0 .. (cons an nil) ..) mc
+                     (fun tr' mem' rets mc' =>
                         rets = nil /\ post))) ..))
     (at level 200,
      name at level 0,
      a0 binder, an binder,
-     tr name, tr' name, mem name, mem' name,
+     tr name, tr' name, mem name, mem' name, mc name, mc' name,
      pre at level 200,
      post at level 200).
 
-Notation "'fnspec!' name '/' g0 .. gn ',' '{' 'requires' tr mem := pre ';' 'ensures' tr' mem' ':=' post '}'" :=
+Notation "'fnspec!' name '/' g0 .. gn ',' '{' 'requires' tr mem mc := pre ';' 'ensures' tr' mem' mc' ':=' post '}'" :=
   (fun functions =>
               (forall g0,
                   .. (forall gn,
-                         (forall tr mem,
+                         (forall tr mem mc,
                              pre ->
                              WeakestPrecondition.call
-                               functions name tr mem nil
-                               (fun tr' mem' rets =>
+                               functions name tr mem nil mc
+                               (fun tr' mem' rets mc' =>
                                   rets = nil /\ post))) ..))
     (at level 200,
      name at level 0,
      g0 binder, gn binder,
-     tr name, tr' name, mem name, mem' name,
+     tr name, tr' name, mem name, mem' name, mc name, mc' name,
      pre at level 200,
      post at level 200).
 
-Notation "'fnspec!' name '~>' r0 .. rn ',' '{' 'requires' tr mem := pre ';' 'ensures' tr' mem' ':=' post '}'" :=
+Notation "'fnspec!' name '~>' r0 .. rn ',' '{' 'requires' tr mem mc := pre ';' 'ensures' tr' mem' mc' ':=' post '}'" :=
   (fun functions =>
-     (forall tr mem,
+     (forall tr mem mc,
          pre ->
          WeakestPrecondition.call
-           functions name tr mem nil
-           (fun tr' mem' rets =>
+           functions name tr mem nil mc
+           (fun tr' mem' rets mc' =>
               (exists r0,
                   .. (exists rn,
                          rets = (cons r0 .. (cons rn nil) ..) /\
@@ -320,6 +337,6 @@ Notation "'fnspec!' name '~>' r0 .. rn ',' '{' 'requires' tr mem := pre ';' 'ens
     (at level 200,
      name at level 0,
      r0 closed binder, rn closed binder,
-     tr name, tr' name, mem name, mem' name,
+     tr name, tr' name, mem name, mem' name, mc name, mc' name,
      pre at level 200,
      post at level 200).
