bedrock2/src/bedrock2/Loops.v
@@ -8,6 +8,8 @@ From bedrock2 Require Import Map.Separation Map.SeparationLogic.
 From bedrock2 Require Import Syntax Semantics Markers.
 From bedrock2 Require Import WeakestPrecondition WeakestPreconditionProperties.
 
+Require Import bedrock2.MetricLogging.
+
 Section Loops.
   Context {width: Z} {BW: Bitwidth width} {word: word.word width} {mem: map.map word Byte.byte}.
   Context {locals: map.map String.string word}.
@@ -81,155 +83,166 @@ Section Loops.
   Import pair.
 
   Lemma while_localsmap
-    {e c t l} {m : mem}
-    {measure : Type} (invariant:_->_->_->_->Prop)
+    {e c t l mc} {m : mem}
+    {measure : Type} (invariant:_->_->_-> _ -> _ -> Prop)
     {lt} (Hwf : well_founded lt) (v0 : measure)
-    {post : _->_->_-> Prop}
-    (Hpre : invariant v0 t m l)
-    (Hbody : forall v t m l,
-      invariant v t m l ->
-      exists br, expr m l e (eq br) /\
+    {post : _->_->_-> _ -> Prop}
+    (Hpre : invariant v0 t m l mc)
+    (Hbody : forall v t m l mc,
+      invariant v t m l mc ->
+      exists br mcnew, expr m l e mc (eq (Datatypes.pair br mcnew)) /\
          (word.unsigned br <> 0 ->
-          cmd call c t m l (fun t m l => exists v', invariant v' t m l /\ lt v' v)) /\
-         (word.unsigned br = 0 -> post t m l))
-    : cmd call (cmd.while e c) t m l post.
+          cmd call c t m l mcnew (fun t m l mcnew' => exists v', invariant v' t m l (addMetricInstructions 2 (addMetricLoads 2 (addMetricJumps 1 mcnew'))) /\ lt v' v)) /\
+         (word.unsigned br = 0 -> post t m l (addMetricInstructions 1 (addMetricLoads 1 (addMetricJumps 1 mcnew)))))
+    : cmd call (cmd.while e c) t m l mc post.
   Proof.
+    
     eexists measure, lt, invariant.
     split. 1: exact Hwf.
     split. 1: eauto.
+    
     exact Hbody.
   Qed.
 
   Lemma while
-    {e c t l} {m : mem}
+    {e c t l mc} {m : mem}
     (variables : list String.string)
     {localstuple : tuple word (length variables)}
-    {measure : Type} (invariant:_->_->_->ufunc word (length variables) Prop)
+    {measure : Type} (invariant:_->_->_->_-> ufunc word (length variables) Prop)
     {lt} (Hwf : well_founded lt) (v0 : measure)
-    {post : _->_->_-> Prop}
+    {post : _->_->_-> _ -> Prop}
     (Pl : enforce variables localstuple l)
-    (Hpre : tuple.apply (invariant v0 t m) localstuple)
-    (Hbody : forall v t m, tuple.foralls (fun localstuple =>
-      tuple.apply (invariant v t m) localstuple ->
+    (Hpre : tuple.apply (invariant v0 t m mc) localstuple)
+    (Hbody : forall v t m mc, tuple.foralls (fun localstuple =>
+      tuple.apply (invariant v t m mc) localstuple ->
       let l := reconstruct variables localstuple in
-      exists br, expr m l e (eq br) /\
+      exists br mcnew, expr m l e mc (eq (Datatypes.pair br mcnew)) /\
          (word.unsigned br <> 0 ->
-          cmd call c t m l (fun t m l =>
+          cmd call c t m l mcnew (fun t m l mcnew' =>
             Markers.unique (Markers.left (tuple.existss (fun localstuple =>
               enforce variables localstuple l /\
               Markers.right (Markers.unique (exists v',
-                tuple.apply (invariant v' t m) localstuple /\ lt v' v))))))) /\
-         (word.unsigned br = 0 -> post t m l)))
-    : cmd call (cmd.while e c) t m l post.
+                tuple.apply (invariant v' t m (addMetricInstructions 2 (addMetricLoads 2 (addMetricJumps 1 mcnew')))) localstuple /\ lt v' v))))))) /\
+         (word.unsigned br = 0 -> post t m l (addMetricInstructions 1 (addMetricLoads 1 (addMetricJumps 1 mcnew))))))
+    : cmd call (cmd.while e c) t m l mc post.
   Proof.
-    eapply (while_localsmap (fun v t m l =>
+    eapply (while_localsmap (fun v t m l mc =>
       exists localstuple, enforce variables localstuple l /\
-                          tuple.apply (invariant v t m) localstuple));
+                          tuple.apply (invariant v t m mc) localstuple));
       unfold Markers.split; eauto.
-    intros vi ti mi li (?&X&Y).
-    specialize (Hbody vi ti mi).
+    intros vi ti mi li mci (?&X&Y).
+    specialize (Hbody vi ti mi mci).
     eapply hlist.foralls_forall in Hbody.
     specialize (Hbody Y).
     rewrite <-(reconstruct_enforce _ _ _ X) in Hbody.
-    destruct Hbody as (br & Cond & Again & Done).
-    exists br. split; [exact Cond|]. split; [|exact Done].
+    destruct Hbody as (br & mcnew & Cond & Again & Done).
+    exists br. exists mcnew. split; [exact Cond|].
+
+    split; [|exact Done].
     intro NE. specialize (Again NE).
     eapply Proper_cmd; [eapply Proper_call| |eapply Again].
     cbv [Morphisms.pointwise_relation Basics.impl Markers.right Markers.unique Markers.left] in *.
-    intros t' m' l' Ex.
+    intros t' m' l' mc' Ex.
     eapply hlist.existss_exists in Ex. cbv beta in Ex. destruct Ex as (ls & E & v' & Inv' & LT).
     eauto.
   Qed.
 
   Lemma tailrec
-    {e c t localsmap} {m : mem}
+    {e c t localsmap mc} {m : mem}
     (ghosttypes : polymorphic_list.list Type)
     (variables : list String.string)
     {l0 : tuple word (length variables)}
     {Pl : enforce variables l0 localsmap}
-    {post : _->_->_-> Prop}
-    {measure : Type} (spec:_->HList.arrows ghosttypes (_->_->ufunc word (length variables) (Prop*(_->_->ufunc word (length variables) Prop)))) lt
+    {post : _->_->_->_-> Prop}
+    {measure : Type} (spec:_->HList.arrows ghosttypes (_->_->ufunc word (length variables) (MetricLog -> Prop*(_->_->ufunc word (length variables) (MetricLog -> Prop))))) lt
     (Hwf : well_founded lt)
     (v0 : measure)
     : hlist.foralls (fun (g0 : hlist ghosttypes) => forall
-    (Hpre : (tuple.apply (hlist.apply (spec v0) g0 t m) l0).(1))
-    (Hbody : forall v, hlist.foralls (fun g => forall t m, tuple.foralls (fun l =>
+                         (Hpre : (tuple.apply (hlist.apply (spec v0) g0 t m) l0 mc).(1))
+                
+    (Hbody : forall v, hlist.foralls (fun g => forall t m mc, tuple.foralls (fun l =>
       @dlet _ (fun _ => Prop) (reconstruct variables l) (fun localsmap : locals =>
-      match tuple.apply (hlist.apply (spec v) g t m) l with S_ =>
+      match tuple.apply (hlist.apply (spec v) g t m) l mc with S_ =>
       S_.(1) ->
-      Markers.unique (Markers.left (exists br, expr m localsmap e (eq br) /\ Markers.right (
-      (word.unsigned br <> 0%Z -> cmd call c t m localsmap
-        (fun t' m' localsmap' =>
+      Markers.unique (Markers.left (exists br mc', expr m localsmap e mc (eq (Datatypes.pair br mc')) /\ Markers.right (
+      (word.unsigned br <> 0%Z -> cmd call c t m localsmap mc'
+        (fun t' m' localsmap' mc'' =>
           Markers.unique (Markers.left (hlist.existss (fun l' => enforce variables l' localsmap' /\ Markers.right (
           Markers.unique (Markers.left (hlist.existss (fun g' => exists v',
-          match tuple.apply (hlist.apply (spec v') g' t' m') l' with S' =>
+          match tuple.apply (hlist.apply (spec v') g' t' m') l' (addMetricInstructions 2 (addMetricLoads 2 (addMetricJumps 1 mc''))) with S' =>
           S'.(1) /\ Markers.right (
             lt v' v /\
-            forall T M, hlist.foralls (fun L => tuple.apply (S'.(2) T M) L -> tuple.apply (S_.(2) T M) L)) end))))))))) /\
-      (word.unsigned br = 0%Z -> tuple.apply (S_.(2) t m) l))))end))))
-    (Hpost : match (tuple.apply (hlist.apply (spec v0) g0 t m) l0).(2) with Q0 => forall t m, hlist.foralls (fun l =>  tuple.apply (Q0 t m) l -> post t m (reconstruct variables l))end)
-    , cmd call (cmd.while e c) t m localsmap post ).
+            forall T M, hlist.foralls (fun L => forall MC, tuple.apply (S'.(2) T M) L MC -> tuple.apply (S_.(2) T M) L MC)) end))))))))) /\
+      (word.unsigned br = 0%Z -> tuple.apply (S_.(2) t m) l (addMetricInstructions 1 (addMetricLoads 1 (addMetricJumps 1 mc')))))))end))))
+    (Hpost : match (tuple.apply (hlist.apply (spec v0) g0 t m) l0 mc).(2) with Q0 => forall t m mc, hlist.foralls (fun l =>  tuple.apply (Q0 t m) l mc -> post t m (reconstruct variables l) mc)end)
+    , cmd call (cmd.while e c) t m localsmap mc post ).
   Proof.
     eapply hlist_forall_foralls; intros g0 **.
-    eexists measure, lt, (fun vi ti mi localsmapi =>
+    eexists measure, lt, (fun vi ti mi localsmapi mci =>
       exists gi li, localsmapi = reconstruct variables li /\
-      match tuple.apply (hlist.apply (spec vi) gi ti mi) li with S_ =>
-      S_.(1) /\ forall T M L, tuple.apply (S_.(2) T M) L ->
-        tuple.apply ((tuple.apply (hlist.apply (spec v0) g0 t m) l0).(2) T M) L end).
+      match tuple.apply (hlist.apply (spec vi) gi ti mi) li mci with S_ =>
+      S_.(1) /\ forall T M L MC, tuple.apply (S_.(2) T M) L MC->
+        tuple.apply ((tuple.apply (hlist.apply (spec v0) g0 t m) l0 mc).(2) T M) L MC end).
     cbv [Markers.split Markers.left Markers.right] in *.
     split; [assumption|].
     split. { exists v0, g0, l0. split. 1: eapply reconstruct_enforce; eassumption. split; eauto. }
-    intros vi ti mi lmapi (gi&?&?&?&Qi); subst.
-    destruct (hlist.foralls_forall (hlist.foralls_forall (Hbody vi) gi ti mi) _ ltac:(eassumption)) as (br&?&X).
-    exists br; split; [assumption|]. destruct X as (Htrue&Hfalse). split; intros Hbr;
+    intros vi ti mi lmapi mci (gi&?&?&?&Qi); subst.
+    destruct (hlist.foralls_forall (hlist.foralls_forall (Hbody vi) gi ti mi mci) _ ltac:(eassumption)) as (br&?&?&X).
+
+      
+    exists br; exists x0; split; [assumption|]. destruct X as (Htrue&Hfalse). split; intros Hbr;
       [pose proof(Htrue Hbr)as Hpc|pose proof(Hfalse Hbr)as Hpc]; clear Hbr Htrue Hfalse.
     { eapply Proper_cmd; [reflexivity..| | |eapply Hpc].
       { eapply Proper_call; firstorder idtac. }
-      intros tj mj lmapj Hlj; eapply hlist.existss_exists in Hlj.
+      intros tj mj lmapj mcj Hlj; eapply hlist.existss_exists in Hlj.
       destruct Hlj as (lj&Elj&HE); eapply reconstruct_enforce in Elj; subst lmapj.
       eapply hlist.existss_exists in HE. destruct HE as (l&?&?&?&HR).
       pose proof fun T M => hlist.foralls_forall (HR T M); clear HR.
       eauto 9. }
-    { pose proof fun t m => hlist.foralls_forall (Hpost t m); clear Hpost; eauto. }
+    { pose proof fun t m mc => hlist.foralls_forall (Hpost t m mc); clear Hpost; eauto. }
   Qed.
 
   Lemma tailrec_localsmap
-    {e c t} {m : mem} {l} {post : _->_->_-> Prop}
-    {measure : Type} (spec:_->_->_->_->(Prop*(_->_->_-> Prop))) lt
+    {e c t} {m : mem} {l mc} {post : _ -> _->_->_-> Prop}
+    {measure : Type} (spec:_->_->_->_->_->(Prop*(_->_->_->_-> Prop))) lt
     (Hwf : well_founded lt)
-    (v0 : measure) (P0 := (spec v0 t m l).(1)) (Hpre : P0)
-    (Q0 := (spec v0 t m l).(2))
-    (Hbody : forall v t m l,
-      let S := spec v t m l in let (P, Q) := S in
+    (v0 : measure) (P0 := (spec v0 t m l mc).(1)) (Hpre : P0)
+    (Q0 := (spec v0 t m l mc).(2))
+    (Hbody : forall v t m l mc,
+      let S := spec v t m l mc in let (P, Q) := S in
       P ->
-      exists br, expr m l e (eq br) /\
-      (word.unsigned br <> 0%Z -> cmd call c t m l
-        (fun t' m' l' => exists v',
-          let S' := spec v' t' m' l' in let '(P', Q') := S' in
+      exists br mc', expr m l e mc (eq (Datatypes.pair br mc')) /\
+      (word.unsigned br <> 0%Z -> cmd call c t m l mc'
+        (fun t' m' l' mc''=> exists v',
+          let S' := spec v' t' m' l' (addMetricInstructions 2
+                                     (addMetricLoads 2
+                                     (addMetricJumps 1 mc''))) in let '(P', Q') := S' in
           P' /\
           lt v' v /\
-          forall T M L, Q' T M L -> Q T M L)) /\
-      (word.unsigned br = 0%Z -> Q t m l))
-    (Hpost : forall t m l, Q0 t m l -> post t m l)
-    : cmd call (cmd.while e c) t m l post.
+          forall T M L MC, Q' T M L MC -> Q T M L MC)) /\
+      (word.unsigned br = 0%Z -> Q t m l (addMetricInstructions 1
+                                         (addMetricLoads 1
+                                         (addMetricJumps 1 mc')))))
+    (Hpost : forall t m l mc, Q0 t m l mc -> post t m l mc)
+    : cmd call (cmd.while e c) t m l mc post.
   Proof.
-    eexists measure, lt, (fun v t m l =>
-      let S := spec v t m l in let '(P, Q) := S in
-      P /\ forall T M L, Q T M L -> Q0 T M L).
+    eexists measure, lt, (fun v t m l mc =>
+      let S := spec v t m l mc in let '(P, Q) := S in
+      P /\ forall T M L MC, Q T M L MC -> Q0 T M L MC).
     split; [assumption|].
     cbv [Markers.split] in *.
     split; [solve[eauto]|].
-    intros vi ti mi li (?&Qi).
-    destruct (Hbody _ _ _ _ ltac:(eassumption)) as (br&?&X); exists br; split; [assumption|].
+    intros vi ti mi li mci (?&Qi).
+    destruct (Hbody _ _ _ _ _ ltac:(eassumption)) as (br&?&?&X); exists br; eexists; split; [eassumption|].
     destruct X as (Htrue&Hfalse). split; intros Hbr;
       [pose proof(Htrue Hbr)as Hpc|pose proof(Hfalse Hbr)as Hpc]; clear Hbr Htrue Hfalse.
     { eapply Proper_cmd; [reflexivity..| | |eapply Hpc].
       { eapply Proper_call; firstorder idtac. }
-      intros tj mj lj (vj&dP&?&dQ); eauto 9. }
+      intros tj mj lj mcj (vj&dP&?&dQ); eauto 9. }
     { eauto. }
   Qed.
 
-  Definition with_bottom {T} R (x y : option T) :=
+   Definition with_bottom {T} R (x y : option T) :=
     match x, y with
     | None, Some _ => True
     | Some x, Some y => R x y
@@ -243,37 +256,70 @@ Section Loops.
     constructor. intros [y|] pf; eauto.
     constructor. intros [] [].
   Qed.
-
-
+  
   Lemma atleastonce_localsmap
-    {e c t} {m : mem} {l} {post : _->_->_-> Prop}
-    {measure : Type} (invariant:_->_->_->_->Prop) lt
+    {e c t} {m : mem} {l mc} {post : _->_->_->_-> Prop}
+    {measure : Type} (invariant:_->_->_->_->_->Prop) lt
     (Hwf : well_founded lt)
-    (Henter : exists br, expr m l e (eq br) /\ (word.unsigned br = 0%Z -> post t m l))
-    (v0 : measure) (Hpre : invariant v0 t m l)
-    (Hbody : forall v t m l, invariant v t m l ->
-       cmd call c t m l (fun t m l =>
-         exists br, expr m l e (eq br) /\
-         (word.unsigned br <> 0 -> exists v', invariant v' t m l /\ lt v' v) /\
-         (word.unsigned br =  0 -> post t m l)))
-    : cmd call (cmd.while e c) t m l post.
+    (Henter : exists br mc', expr m l e mc (eq (Datatypes.pair br mc')) /\ (word.unsigned br = 0%Z -> post t m l (addMetricInstructions 1
+                                         (addMetricLoads 1
+                                            (addMetricJumps 1 mc'))))
+    /\ (word.unsigned br <> 0 -> exists v', invariant v' t m l (addMetricInstructions 2
+                                         (addMetricLoads 2
+                                            (addMetricJumps 1 mc'))))
+    )
+    (v0 : measure) (Hpre : invariant v0 t m l mc)
+    (Hbody : forall v t m l mc, invariant v t m l mc ->
+                                cmd call c t m l mc (fun t m l mc =>
+         exists br mc', expr m l e mc (eq (Datatypes.pair br mc')) /\
+         (word.unsigned br <> 0 -> exists v', invariant v' t m l (addMetricInstructions 2
+                                     (addMetricLoads 2
+                                     (addMetricJumps 1 mc'))) /\ lt v' v) /\
+         (word.unsigned br =  0 -> post t m l (addMetricInstructions 1
+                                         (addMetricLoads 1
+                                         (addMetricJumps 1 mc'))))))
+    : cmd call (cmd.while e c) t m l mc post.
   Proof.
-    eexists (option measure), (with_bottom lt), (fun ov t m l =>
-      exists br, expr m l e (eq br) /\
-      ((word.unsigned br <> 0 -> exists v, ov = Some v /\ invariant v t m l) /\
-      (word.unsigned br =  0 -> ov = None /\ post t m l))).
+    eexists (option measure), (with_bottom lt), (fun ov t m l mc =>
+      exists br mc', expr m l e mc (eq (Datatypes.pair br mc')) /\
+      ((word.unsigned br <> 0 -> exists v, ov = Some v /\ invariant v t m l (addMetricInstructions 2
+                                     (addMetricLoads 2
+                                     (addMetricJumps 1 mc')))) /\
+      (word.unsigned br =  0 -> ov = None /\ post t m l (addMetricInstructions 1
+                                         (addMetricLoads 1
+                                         (addMetricJumps 1 mc')))))).
     split; auto using well_founded_with_bottom; []. split.
-    { destruct Henter as [br [He Henter]].
+    { destruct Henter as [br [mc' [He [Henter0 Henterm]]]].
       destruct (BinInt.Z.eq_dec (word.unsigned br) 0).
-      { exists None, br; split; trivial.
+      { exists None, br, mc'; split; trivial.
         split; intros; try contradiction; split; eauto. }
-      { exists (Some v0), br.
+      {
+        assert (Hnonzero := n).
+        apply Henterm in Hnonzero. 
+        destruct Hnonzero as [v Hinv].
+        exists (Some v), br, mc'.
+
         split; trivial; []; split; try contradiction.
-        exists v0; split; trivial. } }
-    intros vi ti mi li (br&Ebr&Hcontinue&Hexit).
-    eexists; split; [eassumption|]; split.
-    { intros Hc; destruct (Hcontinue Hc) as (v&?&Hinv); subst.
-      eapply Proper_cmd; [| |eapply Hbody; eassumption]; [eapply Proper_call|].
+
+        exists v; split; trivial. 
+
+
+    } }
+    intros vi ti mi li mci (br&mcnew&Ebr&Hcontinue&Hexit).
+    eexists; eexists; split.
+    - eassumption.
+    - split.
+      
+    
+    (*eexists; eexists; split; [eassumption|]; split.*)
+
+    { 
+      intros Hc; destruct (Hcontinue Hc) as (v&?&Hinv); subst.
+      eapply Proper_cmd.
+      1: { eapply Proper_call. }
+      2: { (* eapply Hbody. eassumption. }
+
+      [ | | eapply Hbody; eassumption]. [eapply Proper_call|].
       intros t' m' l' (br'&Ebr'&Hinv'&Hpost').
       destruct (BinInt.Z.eq_dec (word.unsigned br') 0).
       { exists None; split; try constructor.
@@ -285,26 +331,80 @@ Section Loops.
         exists br'; split; trivial.
         split; intros; try contradiction.
         eexists; split; eauto. } }
+    
     eapply Hexit.
-  Qed.
+  Qed. 
+         *) Admitted.
+    
+  Lemma atleastonce
+    {e c t l mc} {m : mem}
+    (variables : list String.string)
+    {localstuple : tuple word (length variables)}
+    {Pl : enforce variables localstuple l}
+    {measure : Type} (invariant:_->_->_-> ufunc word (length variables) (MetricLog -> Prop))
+    lt (Hwf : well_founded lt)
+    {post : _->_->_->_->Prop}
+    (Henter : exists br mc', expr m l e mc (eq (Datatypes.pair br mc')) /\ (word.unsigned br = 0%Z -> post t m l (addMetricInstructions 1
+                                         (addMetricLoads 1
+                                            (addMetricJumps 1 mc')))) /\
+                                          (word.unsigned br <> 0 -> exists v', tuple.apply (invariant v' t m) localstuple (addMetricInstructions 2
+                                         (addMetricLoads 2
+                                            (addMetricJumps 1 mc'))))
 
+    )
+    (v0 : measure) (Hpre : tuple.apply (invariant v0 t m) localstuple mc)
+    (Hbody : forall v t m mc, tuple.foralls (fun localstuple =>
+      tuple.apply (invariant v t m) localstuple mc ->
+       cmd call c t m (reconstruct variables localstuple) mc (fun t m l mc =>
+         exists br mc', expr m l e mc (eq (Datatypes.pair br mc')) /\
+         (word.unsigned br <> 0 -> Markers.unique (Markers.left (tuple.existss (fun localstuple => enforce variables localstuple l /\ Markers.right (Markers.unique (exists v', tuple.apply (invariant v' t m) localstuple (addMetricInstructions 2
+                                     (addMetricLoads 2
+                                     (addMetricJumps 1 mc'))) /\ lt v' v)))))) /\
+         (word.unsigned br =  0 -> post t m l (addMetricInstructions 1
+                                         (addMetricLoads 1
+                                         (addMetricJumps 1 mc')))))))
+    : cmd call (cmd.while e c) t m l mc post.
+  Proof.
+    eapply (atleastonce_localsmap (fun v t m l mc => exists localstuple, Logic.and (enforce variables localstuple l) (tuple.apply (invariant v t m) localstuple mc))); eauto.
+    {
+      destruct Henter as [br0 [mc0 [Henter [Henter0 Henternonzero]]]].
+      exists br0. exists mc0. repeat (split; eauto).
+      intro Hnonzero. apply Henternonzero in Hnonzero. destruct Hnonzero as [v Hnonzero].
+      exists v. exists localstuple. repeat (split; eauto).
+    }
+    { 
+    intros vi ti mi li mci (?&X&Y).
+    specialize (Hbody vi ti mi).
+    eapply hlist.foralls_forall in Hbody.
+    specialize (Hbody Y).
+    rewrite <-(reconstruct_enforce _ _ _ X) in Hbody.
+    eapply Proper_cmd; [eapply Proper_call| |eapply Hbody].
+    intros t' m' l' mc' (?&?&?&HH).
+    eexists; eexists; split; eauto. destruct HH as [HH1 HH2].
+    split; intros; eauto.
+    specialize (HH1 ltac:(eauto)).
+    eapply hlist.existss_exists in HH1; destruct HH1 as (?&?&?&?&?).
+    eexists; split; eauto.
+    }
+  Qed.
+  (*
   Lemma tailrec_earlyout_localsmap
-    {e c t} {m : mem} {l} {post : _->_->_-> Prop}
-    {measure : Type} (spec:_->_->_->_->(Prop*(_->_->_-> Prop))) lt
+    {e c t} {m : mem} {l mc} {post : _-> _->_->_-> Prop}
+    {measure : Type} (spec:_->_->_->_->_->(Prop*(_->_->_->_-> Prop))) lt
     (Hwf : well_founded lt)
-    (v0 : measure) (P0 := (spec v0 t m l).(1)) (Hpre : P0)
-    (Q0 := (spec v0 t m l).(2))
-    (Hbody : forall v t m l,
-      let S := spec v t m l in let (P, Q) := S in
+    (v0 : measure) (P0 := (spec v0 t m l mc).(1)) (Hpre : P0)
+    (Q0 := (spec v0 t m l mc).(2))
+    (Hbody : forall v t m l mc,
+      let S := spec v t m l mc in let (P, Q) := S in
       P ->
-      exists br, expr m l e (eq br) /\
-      (word.unsigned br <> 0%Z -> cmd call c t m l
-        (fun t' m' l' =>
-          (exists br, expr m' l' e (eq br) /\ word.unsigned br = 0 /\ Q t' m' l') \/
+      exists br mc', expr m l e mc (eq (Datatypes.pair br mc')) /\
+      (word.unsigned br <> 0%Z -> cmd call c t m l mc'
+        (fun t' m' l' mc'' =>
+          (exists br mc', expr m' l' e mc'' (eq (Datatypes.pair br mc')) /\ word.unsigned br = 0 /\ Q t' m' l' mc') \/
           exists v', let S' := spec v' t' m' l' in let '(P', Q') := S' in
           P' /\
           lt v' v /\
-          forall T M L, Q' T M L -> Q T M L)) /\
+          forall T M L MC, Q' T M L -> Q T M L)) /\
       (word.unsigned br = 0%Z -> Q t m l))
     (Hpost : forall t m l, Q0 t m l -> post t m l)
     : cmd call (cmd.while e c) t m l post.
@@ -391,40 +491,6 @@ Section Loops.
     { pose proof fun t m => hlist.foralls_forall (Hpost t m); clear Hpost; eauto. }
   Qed.
 
-
-  Lemma atleastonce
-    {e c t l} {m : mem}
-    (variables : list String.string)
-    {localstuple : tuple word (length variables)}
-    {Pl : enforce variables localstuple l}
-    {measure : Type} (invariant:_->_->_->ufunc word (length variables) Prop)
-    lt (Hwf : well_founded lt)
-    {post : _->_->_-> Prop}
-    (Henter : exists br, expr m l e (eq br) /\ (word.unsigned br = 0%Z -> post t m l))
-    (v0 : measure) (Hpre : tuple.apply (invariant v0 t m) localstuple)
-    (Hbody : forall v t m, tuple.foralls (fun localstuple =>
-      tuple.apply (invariant v t m) localstuple ->
-       cmd call c t m (reconstruct variables localstuple) (fun t m l =>
-         exists br, expr m l e (eq br) /\
-         (word.unsigned br <> 0 -> Markers.unique (Markers.left (tuple.existss (fun localstuple => enforce variables localstuple l /\ Markers.right (Markers.unique (exists v', tuple.apply (invariant v' t m) localstuple /\ lt v' v)))))) /\
-         (word.unsigned br =  0 -> post t m l))))
-    : cmd call (cmd.while e c) t m l post.
-  Proof.
-    eapply (atleastonce_localsmap (fun v t m l => exists localstuple, Logic.and (enforce variables localstuple l) (tuple.apply (invariant v t m) localstuple))); eauto.
-    intros vi ti mi li (?&X&Y).
-    specialize (Hbody vi ti mi).
-    eapply hlist.foralls_forall in Hbody.
-    specialize (Hbody Y).
-    rewrite <-(reconstruct_enforce _ _ _ X) in Hbody.
-    eapply Proper_cmd; [eapply Proper_call| |eapply Hbody].
-    intros t' m' l' (?&?&HH&?).
-    eexists; split; eauto.
-    split; intros; eauto.
-    specialize (HH ltac:(eauto)).
-    eapply hlist.existss_exists in HH; destruct HH as (?&?&?&?&?).
-    eexists; split; eauto.
-  Qed.
-
   Lemma while_zero_iterations {e c t l} {m : mem} {post : _->_->_-> Prop}
     (HCond: expr m l e (eq (word.of_Z 0)))
     (HPost: post t m l)
@@ -473,6 +539,7 @@ Section Loops.
       intros. rewrite (sep_comm _ dR), <-(sep_assoc _ dR), dQ; trivial. }
     { eapply Hpost, Qi, Hpc. }
   Qed.
+*)
 End Loops.
 
 Ltac loop_simpl :=
@@ -483,3 +550,4 @@ Ltac loop_simpl :=
        List.repeat Datatypes.length
        HList.polymorphic_list.repeat HList.polymorphic_list.length
        PrimitivePair.pair._1 PrimitivePair.pair._2] in *.
+
